theories/rules/mem_retrieve.v
@@ -97,7 +97,6 @@ Proof.
   }
 Qed.
 
-
 Lemma mem_retrieve_donate {E i wi sacc p_tx r0 sh j mem_rx p_rx} {ps: gset PID} ai wh:
   (* has access to the page which the instruction is in *)
   tpa ai ≠ p_tx ->
@@ -143,6 +142,217 @@ Lemma mem_retrieve_donate {E i wi sacc p_tx r0 sh j mem_rx p_rx} {ps: gset PID} 
        (* the transaction is completed, deallocate it and release the handle *)
        fresh_handles 1 (sh ∪ {[wh]}) }}}.
 Proof.
+  iIntros (Hneq_tx Hin_acc Hdecode_i Hdecode_f Φ)
+          "(>PC & >mem_ins & >R0 & >R1 & >own &>acc & >tx & >re & >tran & >rx & >rx_s & >mem_rx & >[hp handles]) HΦ".
+  iApply (sswp_lift_atomic_step ExecI);[done|].
+  iIntros (n σ1) "%Hsche state".
+  rewrite /scheduled /= /scheduler in Hsche.
+  assert (σ1.1.1.2 = i) as Heq_cur. { case_bool_decide;last done. by apply fin_to_nat_inj. }
+  clear Hsche.
+  iModIntro.
+  iDestruct "state" as "(Hnum & mem & regs & mb & rx_state & pgt_owned & pgt_acc & pgt_excl &
+                            trans & hpool & retri & %Hwf & %Hdisj & %Hconsis )".
+  (* valid regs *)
+  iDestruct ((gen_reg_valid3 i PC ai R0 r0 R1 wh Heq_cur) with "regs PC R0 R1")
+    as "(%Hlookup_PC & %Hlookup_R0 & %Hlookup_R1)";eauto.
+  (* valid pt *)
+  iDestruct (access_agree_check_true (tpa ai) i with "pgt_acc acc") as %Hcheckpg_ai;eauto.
+  (* valid mem *)
+  iDestruct (gen_mem_valid ai wi with "mem mem_ins") as %Hlookup_ai.
+  iDestruct (gen_mem_valid_SepM_subseteq with "mem [mem_rx]") as %Hsubseteq_mem_rx.
+  { iDestruct "mem_rx" as "[% mem_rx]". iExact "mem_rx". }
+  (* valid tx rx *)
+  iDestruct (mb_valid_tx i p_tx with "mb tx") as %Heq_tx.
+  iDestruct (mb_valid_rx i p_rx with "mb rx") as %Heq_rx.
+  iDestruct (rx_state_valid_None with "rx_state rx_s") as %Heq_rx_state.
+  (* valid trans *)
+  iDestruct (trans_valid_Some with "trans tran") as %[re Hlookup_tran].
+  iDestruct (retri_valid_Some with "retri re") as %[meta Hlookup_tran'].
+  rewrite Hlookup_tran in Hlookup_tran'.
+  inversion Hlookup_tran'. subst re. clear meta Hlookup_tran' H1.
+  (* valid hpool *)
+  iDestruct (hpool_valid with "hpool hp") as %Heq_hp.
+  (* iAssert ( ⌜wh ∉ sh⌝)%I as %Hnin. { iApply not_elem_of_fresh_handles. iFrame. } *)
+  iSplit.
+  - (* reducible *)
+    iPureIntro.
+    apply (reducible_normal i Hvc ai wi);eauto.
+    rewrite Heq_tx //.
+  - iModIntro.
+    iIntros (m2 σ2) "vmprop_auth %HstepP".
+    iFrame "vmprop_auth".
+    apply (step_ExecI_normal i Hvc ai wi) in HstepP;eauto.
+    2: rewrite Heq_tx //.
+    remember (exec Hvc σ1) as c2 eqn:Heqc2.
+    rewrite /exec /hvc Hlookup_R0 /= Hdecode_f /retrieve Hlookup_R1 /get_transaction /= Hlookup_tran Heq_cur /=  in Heqc2.
+    case_bool_decide;last done. clear H0.
+    assert (is_Some(finz.of_z (finz_bound := word_size) (Z.of_nat (size ps + 4)%nat))) as [l Heq_l].
+    {
+      destruct Hwf as [Hub _].
+      specialize (Hub wh _ Hlookup_tran).
+      simpl in Hub.
+      rewrite Z.leb_le in Hub.
+      apply finz_of_z_is_Some.
+      lia. lia.
+    }
+    rewrite Heq_l Heq_rx in Heqc2.
+    rewrite /fill_rx in Heqc2.
+    assert (Heq_mb: (σ1.1.1.1.1.2 !!! i) = (p_tx, (p_rx, None))).
+    rewrite -Heq_tx -Heq_rx -Heq_rx_state. rewrite -2!surjective_pairing //.
+    rewrite p_wr_mem_mb Heq_mb /= in Heqc2.
+    destruct HstepP;subst m2 σ2; subst c2.
+    rewrite /= /gen_vm_interp.
+    (* unchanged part *)
+    set σ_fill := (fill_rx_unsafe (write_mem_segment σ1 p_rx _) l i i p_tx p_rx).
+    rewrite (preserve_get_mb_gmap σ_fill (update_incr_PC _)).
+    2: rewrite p_upd_pc_mb p_upd_reg_mb p_upd_own_mb p_grnt_acc_mb p_upd_tran_mb //.
+    rewrite p_fill_rx_mb. all : try rewrite p_wr_mem_mb //.
+    rewrite (preserve_get_mb_gmap σ1).
+    2: rewrite p_wr_mem_mb //.
+    iFrame "Hnum mb".
+    (* upd mem *)
+    rewrite p_upd_pc_mem p_upd_reg_mem p_upd_own_mem p_grnt_acc_mem p_upd_tran_mem.
+    rewrite p_fill_rx_mem u_wr_mem_mem.
+    iDestruct "mem_rx" as "[%Hdom_mem_rx mem_rx]".
+    set des := (list_to_map _).
+    assert (Heq_dom : dom (gset Addr) mem_rx = dom (gset Addr) (des ∪ mem_rx)).
+    { symmetry. apply dom_wr_mem_subseteq.
+      destruct Hwf as [Hub _].
+      specialize (Hub wh _ Hlookup_tran).
+      simpl in Hub.
+      rewrite Z.leb_le in Hub.
+      rewrite /= map_length .
+      rewrite /size /set_size /= in Hub. lia.
+      simpl. lia.
+      done.
+    }
+    iDestruct (gen_mem_update_SepM _ (des ∪ mem_rx) with "mem mem_rx") as ">[mem mem_rx]";auto.
+    rewrite -map_union_assoc.
+    assert (mem_rx ∪ σ1.1.2 = σ1.1.2). apply map_subseteq_union. done.
+    iEval (rewrite H0) in "mem". clear H0. iFrame "mem".
+    (* upd regs *)
+    rewrite (u_upd_pc_regs _ i ai). 2: done.
+    2: { rewrite u_upd_reg_regs p_upd_own_current_vm p_grnt_acc_current_vm p_rm_tran_current_vm /σ_fill.
+         rewrite (preserve_get_reg_gmap σ1). rewrite lookup_insert_ne. solve_reg_lookup. done. f_equal.
+    }
+    rewrite u_upd_reg_regs p_upd_own_current_vm p_grnt_acc_current_vm p_rm_tran_current_vm p_fill_rx_current_vm p_wr_mem_current_vm Heq_cur.
+    rewrite (preserve_get_reg_gmap σ1);last done.
+    iDestruct ((gen_reg_update2_global PC i _ (ai ^+ 1)%f R0 i _ (encode_hvc_ret_code Succ)) with "regs PC R0")
+      as ">[$ [PC R0]]";eauto.
+    (* upd pgt *)
+    (* TODO *)
+    (* rewrite (preserve_get_own_gmap (update_page_table_global grant_access (update_transaction σ_fill wh (j, i, ps, Lending, true)) i ps) (update_incr_PC _)). *)
+    (* 2: rewrite p_upd_pc_pgt p_upd_reg_pgt //. *)
+    (* rewrite p_grnt_acc_own. rewrite (preserve_get_own_gmap σ1);last done. *)
+    (* iFrame "pgt_owned". *)
+    (* rewrite (preserve_get_access_gmap (update_page_table_global grant_access (update_transaction σ_fill wh (j, i, ps, Lending, true)) i ps) (update_incr_PC _)). *)
+    (* 2: rewrite p_upd_pc_pgt p_upd_reg_pgt //. *)
+    (* iDestruct (access_agree with "pgt_acc acc") as %Hlookup_pgt_acc. *)
+    (* rewrite (u_grnt_acc_acc _ _ _ sacc). *)
+    (* 2: { *)
+    (*   rewrite p_upd_tran_pgt p_fill_rx_pgt p_wr_mem_pgt. *)
+    (*   intros p Hin_p. *)
+    (*   specialize (Hconsis wh _ Hlookup_tran p Hin_p). *)
+    (*   simpl in Hconsis. *)
+    (*   destruct tt. *)
+    (*   done. *)
+    (*   eexists;done. *)
+    (*   eexists;done. *)
+    (* } *)
+    (* 2: rewrite (preserve_get_access_gmap σ1);done. *)
+    (* rewrite (preserve_get_access_gmap σ1);last done. *)
+    (* iDestruct (access_update (ps ∪ sacc) with "pgt_acc acc") as ">[$ acc]". done. *)
+    (* rewrite (preserve_get_excl_gmap (update_page_table_global grant_access (update_transaction σ_fill wh (j, i, ps, Lending, true)) i ps) (update_incr_PC _)). *)
+    (* 2: rewrite p_upd_pc_pgt p_upd_reg_pgt //. *)
+    (* rewrite p_grnt_acc_excl. *)
+    (* 2: { rewrite p_upd_tran_pgt p_fill_rx_pgt p_wr_mem_pgt. specialize (Hconsis wh _ Hlookup_tran). *)
+    (*      intros p Hin. *)
+    (*      specialize (Hconsis p Hin). *)
+    (*      simpl in Hconsis. *)
+    (*      destruct tt. *)
+    (*      contradiction. *)
+    (*      eexists;split;eauto. *)
+    (*      eexists;split;eauto. *)
+    (* } *)
+    (* rewrite (preserve_get_excl_gmap σ1);last done. *)
+    (* iFrame "pgt_excl". *)
+    (* (* upd rx_state *) *)
+    (* rewrite (preserve_get_rx_gmap σ_fill (update_incr_PC _)). *)
+    (* 2: rewrite p_upd_pc_mb p_upd_reg_mb p_grnt_acc_mb //. *)
+    (* rewrite u_fill_rx_rx_state. *)
+    (* rewrite (preserve_get_rx_gmap σ1); last done. *)
+    (* iDestruct (rx_state_update with "rx_state rx_s") as ">[$ rx_s]". *)
+    (* (* upd tran *) *)
+    (* rewrite (preserve_get_trans_gmap (update_transaction σ_fill wh (j, i, ps, tt, true)) (update_incr_PC _)). *)
+    (* 2: rewrite p_upd_pc_trans p_upd_reg_trans //. *)
+    (* rewrite u_upd_tran_trans (preserve_get_trans_gmap σ1);last done. *)
+    (* rewrite insert_id. *)
+    (* 2: rewrite /get_trans_gmap /get_transactions_gmap lookup_fmap Hlookup_tran //=. *)
+    (* iFrame "trans". *)
+    (* (* upd hp *) *)
+    (* rewrite (preserve_get_hpool_gset (update_transaction σ_fill wh (j, i, ps, tt, true)) (update_incr_PC _)). *)
+    (* 2: rewrite p_upd_pc_trans p_upd_reg_trans //. rewrite p_upd_tran_hp. *)
+    (* iFrame "hpool". *)
+    (* (* upd retri *) *)
+    (* rewrite (preserve_get_retri_gmap (update_transaction σ_fill wh (j, i, ps, tt, true)) (update_incr_PC _)). *)
+    (* 2: rewrite p_upd_pc_trans p_upd_reg_trans //. *)
+    (* 2: { rewrite p_fill_rx_trans p_wr_mem_trans. exists (Some (j, i, ps, tt, false)). split;eauto. } *)
+    (* rewrite u_upd_tran_retri. *)
+    (* iDestruct (retri_update_flip with "retri re") as ">[$ re]". *)
+    (* (* inv_trans_wellformed *) *)
+    (* rewrite (preserve_inv_trans_wellformed (update_transaction σ_fill wh (j, i, ps, tt, true))). *)
+    (* 2: rewrite p_upd_pc_trans p_upd_reg_trans //. *)
+    (* iAssert (⌜inv_trans_wellformed (update_transaction σ_fill wh (j, i, ps, tt, true))⌝%I) as "$". iPureIntro. *)
+    (* apply (p_upd_tran_inv_wf σ1 wh);eauto. *)
+    (* (* inv_trans_pgt_consistent *) *)
+    (* rewrite (preserve_inv_trans_pgt_consistent (update_page_table_global grant_access (update_transaction σ_fill wh (j, i, ps, tt, true)) i ps) (update_incr_PC _)). *)
+    (* 2: rewrite p_upd_pc_trans p_upd_reg_trans //. *)
+    (* 2: rewrite p_upd_pc_pgt p_upd_reg_pgt //. *)
+    (* iAssert (⌜inv_trans_pgt_consistent (update_page_table_global grant_access (update_transaction σ_fill wh (j, i, ps, tt, true)) i ps)⌝%I) as "$". iPureIntro. *)
+    (* apply p_retrieve_inv_consist_not_donate;auto. *)
+    (* (* inv_trans_ps_disj *) *)
+    (* rewrite (preserve_inv_trans_ps_disj (update_transaction σ_fill wh (j, i, ps, tt, true))). *)
+    (* 2: rewrite p_upd_pc_trans p_upd_reg_trans //. *)
+    (* iAssert (⌜inv_trans_ps_disj (update_transaction σ_fill wh (j, i, ps, tt, true))⌝%I) as "$". iPureIntro. *)
+    (* eapply p_upd_tran_inv_disj. *)
+    (* rewrite (preserve_inv_trans_ps_disj σ1) //. *)
+    (* rewrite p_fill_rx_trans p_wr_mem_trans //. *)
+    (* done. *)
+    (* (* just_scheduled *) *)
+    (* iModIntro. *)
+    (* rewrite /just_scheduled_vms /just_scheduled. *)
+    (* rewrite /scheduled /machine.scheduler /= /scheduler. *)
+    (* rewrite p_upd_pc_current_vm p_upd_reg_current_vm p_grnt_acc_current_vm p_upd_tran_current_vm p_fill_rx_current_vm p_wr_mem_current_vm. *)
+    (* rewrite Heq_cur. *)
+    (* iSplitL "". *)
+    (* set fl := (filter _ _). *)
+    (* assert (fl = []) as ->. *)
+    (* { *)
+    (*   rewrite /fl. *)
+    (*   induction n. *)
+    (*   - simpl. *)
+    (*     rewrite filter_nil //=. *)
+    (*   - rewrite seq_S. *)
+    (*     rewrite filter_app. *)
+    (*     rewrite IHn. *)
+    (*     simpl. *)
+    (*     rewrite filter_cons_False /=. rewrite filter_nil //. *)
+    (*     rewrite andb_negb_l //. *)
+    (* } *)
+    (* by iSimpl. *)
+    (* (* Φ *) *)
+    (* case_bool_decide;last contradiction. *)
+    (* simpl. iApply "HΦ". *)
+    (* rewrite /fresh_handles. iFrame. *)
+    (* iExists l. *)
+    (* iExists (of_imm (encode_vmid j) :: wh :: encode_transaction_type tt :: (l ^- 4)%f :: map of_pid (elements ps)). *)
+    (* iFrame. *)
+    (* iSplit. iPureIntro. *)
+    (* simpl. rewrite fmap_length. *)
+    (* rewrite /size /set_size /= in Heq_l. *)
+    (* solve_finz. *)
+    (* iSplit. done. *)
+    (* rewrite -Hdom_mem_rx Heq_dom //. *)
 Admitted.
 
 Lemma mem_retrieve_donate_rx {E i wi sacc r0 sh j mem_rx p_tx} {ps: gset PID} ai wh:
